Finish proof of confluence for red1 without context fixing.

pcuic/theories/PCUICConfluence.v
@@ -164,14 +164,17 @@ Section RedPred.
     now rewrite !subst_ids in X1.
   Qed.
 
+  Ltac noconf H := repeat (DepElim.noconf H; simpl NoConfusion in * ).
+
+
+
   Lemma red1_pred1 Γ : forall M N, red1 Σ Γ M N -> pred1 Σ Γ Γ M N.
   Proof with pcuic.
     induction 1 using red1_ind_all; intros; pcuic.
-    - constructor; pcuic.
-      unfold on_Trel_eq, on_Trel.
+    - econstructor; pcuic. eauto.
+      unfold on_Trel.
       (* TODO fix OnOne2 use in red1 to use onTrel_eq to have equality on annotation *)
-      eapply OnOne2_All2 ... intros x y X0. simpl in X0.
-      intuition auto. admit.
+      eapply OnOne2_All2 ...
     - constructor; pcuic.
       eapply OnOne2_All2...
     - constructor; pcuic.
@@ -179,12 +182,11 @@ Section RedPred.
         now intros; eapply weakening_pred1_pred1.
         (* Missing name equality *)
         eapply OnOne2_All2...
-        intros. unfold on_Trel_eq, on_Trel.
-        simpl in *. intuition auto.
-        admit.
+        intros.
+        simpl in *. intuition auto. now noconf b.
       + eapply OnOne2_All2; pcuic; simpl;
-        unfold on_Trel_eq, on_Trel;
-        intuition auto. rewrite b0; pcuic.
+        unfold on_Trel; simpl; intros; intuition auto.
+        noconf b; noconf H. rewrite H0. pcuic.
         apply pred1_refl_gen.
         eapply All2_local_env_app_inv; pcuic.
         apply All2_All2_local_env_fix_context.
@@ -192,9 +194,9 @@ Section RedPred.
         (* Missing name equality *)
         eapply OnOne2_All2...
         intros.
-        intros. unfold on_Trel_eq, on_Trel.
+        intros. unfold on_Trel.
         simpl in *. intuition auto.
-        admit. admit.
+        congruence. congruence.
 
         pcuic.
         apply pred1_refl_gen; pcuic.
@@ -204,9 +206,8 @@ Section RedPred.
         (* Missing name equality *)
         eapply OnOne2_All2...
         intros.
-        intros. unfold on_Trel_eq, on_Trel.
-        simpl in *. intuition auto.
-        admit.
+        intros. unfold on_Trel.
+        simpl in *. intuition auto. congruence.
 
     - constructor; pcuic.
       apply All2_All2_local_env_fix_context.
@@ -214,48 +215,52 @@ Section RedPred.
       (* Missing name equality *)
       + eapply OnOne2_All2...
         intros.
-        intros. unfold on_Trel_eq, on_Trel.
-        simpl in *. intuition auto.
-        rewrite b0; pcuic. admit.
+        intros. unfold on_Trel.
+        simpl in *. intuition auto. noconf b. noconf H.
+        rewrite H0; pcuic. congruence.
       + eapply OnOne2_All2...
         intros.
-        * intros. unfold on_Trel_eq, on_Trel.
-          simpl in *. intuition auto.
-          rewrite b0; pcuic.
+        * intros. unfold on_Trel.
+          simpl in *. intuition auto. noconf b. noconf H. rewrite H0. pcuic.
           assert(fix_context mfix0 = fix_context mfix1).
           clear -X.
           unfold fix_context, mapi. generalize 0 at 2 4.
-          induction X; intros. intuition auto. simpl. rewrite b0. do 3 f_equal.  admit.
+          induction X; intros. intuition auto. simpl.
+          noconf b. noconf H. now rewrite H H0.
           simpl; now rewrite IHX.
-          now rewrite -H. admit.
-        * intros. unfold on_Trel_eq, on_Trel.
+          now rewrite -H. congruence.
+        * intros. unfold on_Trel.
           simpl in *. intuition pcuic.
           assert(fix_context mfix0 = fix_context mfix1).
           clear -X.
           unfold fix_context, mapi. generalize 0 at 2 4.
-          induction X; intros. intuition auto. simpl. rewrite b0. do 3 f_equal.  admit.
+          induction X; intros. intuition auto. simpl.
+          noconf b; noconf H. now rewrite H H0.
           simpl; now rewrite IHX.
           rewrite -H. pcuic.
 
     - constructor; pcuic.
       apply All2_All2_local_env_fix_context.
       now intros; eapply weakening_pred1_pred1.
+      (* Missing name equality *)
       + eapply OnOne2_All2...
-        unfold on_Trel_eq, on_Trel.
-        simpl in *. intuition pcuic. admit.
+        intros.
+        intros. unfold on_Trel.
+        simpl in *. intuition auto. noconf b. noconf H.
+        rewrite H; pcuic.
       + eapply OnOne2_All2...
-        * unfold on_Trel_eq, on_Trel.
-          simpl in *. intuition pcuic. rewrite -b0; pcuic.
+        * unfold on_Trel.
+          simpl in *. intuition pcuic. noconf b; noconf H.
+          rewrite -H0; pcuic.
           eapply pred1_ctx_pred1; pcuic.
           apply fix_context_assumption_context.
           apply All2_local_env_over_app. pcuic.
           apply All2_All2_local_env_fix_context.
           now intros; eapply weakening_pred1_pred1.
           eapply OnOne2_All2...
-          unfold on_Trel_eq, on_Trel.
-          simpl in *. intuition pcuic. admit.
-          admit.
-        * unfold on_Trel_eq, on_Trel.
+          unfold on_Trel.
+          simpl in *. intuition pcuic. congruence. congruence.
+        * unfold on_Trel.
           simpl in *. intuition pcuic.
           eapply pred1_ctx_pred1; pcuic.
           apply fix_context_assumption_context.
@@ -263,26 +268,26 @@ Section RedPred.
           apply All2_All2_local_env_fix_context.
           now intros; eapply weakening_pred1_pred1.
           eapply OnOne2_All2...
-          unfold on_Trel_eq, on_Trel.
-          simpl in *. intuition pcuic. admit.
+          unfold on_Trel.
+          simpl in *. intuition pcuic. congruence.
 
     - constructor; pcuic.
       apply All2_All2_local_env_fix_context.
       now intros; eapply weakening_pred1_pred1.
       + eapply OnOne2_All2...
-        unfold on_Trel_eq, on_Trel.
-        simpl in *. intuition pcuic. rewrite b0; pcuic.
-        admit.
+        unfold on_Trel.
+        simpl in *. intuition pcuic. noconf b; noconf H; rewrite H0; pcuic.
+        congruence.
       + eapply OnOne2_All2...
-        * unfold on_Trel_eq, on_Trel.
-          simpl in *. intuition pcuic. rewrite -b0; pcuic.
+        * unfold on_Trel.
+          simpl in *. intuition pcuic. noconf b; noconf H; rewrite H0; pcuic.
           assert(fix_context mfix0 = fix_context mfix1).
           { clear -X.
             unfold fix_context, mapi. generalize 0 at 2 4.
-            induction X; intros. intuition auto. simpl. rewrite b0. do 3 f_equal.  admit.
+            induction X; intros. intuition auto. simpl. noconf b; noconf H. congruence.
             simpl; now rewrite IHX. }
-          now rewrite -H. admit.
-        * unfold on_Trel_eq, on_Trel.
+          now rewrite -H. congruence.
+        * unfold on_Trel.
           simpl in *. intuition pcuic.
           eapply pred1_ctx_pred1; pcuic.
           apply fix_context_assumption_context.
@@ -290,8 +295,641 @@ Section RedPred.
           apply All2_All2_local_env_fix_context.
           now intros; eapply weakening_pred1_pred1.
           eapply OnOne2_All2...
-          unfold on_Trel_eq, on_Trel.
-          simpl in *. intuition pcuic. rewrite b0; pcuic. admit.
-  Admitted.
+          unfold on_Trel.
+          simpl in *. intuition pcuic.
+          noconf b; noconf H; rewrite H0; pcuic. congruence.
+  Qed.
 
 End RedPred.
+
+Existing Instance default_checker_flags.
+
+Section PredRed.
+  Context {Σ : global_context}.
+  Context (wfΣ : wf Σ).
+
+  Lemma weakening_red_0 Γ Γ' M N n :
+    n = #|Γ'| ->
+    red Σ Γ M N ->
+    red Σ (Γ ,,, Γ') (lift0 n M) (lift0 n N).
+  Proof. now move=> ->; apply (weakening_red Σ Γ [] Γ'). Qed.
+
+  Lemma red_abs_alt Γ na M M' N N' : red Σ Γ M M' -> red Σ (Γ ,, vass na M) N N' ->
+                                 red Σ Γ (tLambda na M N) (tLambda na M' N').
+  Proof.
+    intros. eapply (transitivity (y := tLambda na M N')).
+    now eapply (red_ctx (tCtxLambda_r _ _ tCtxHole)).
+    now eapply (red_ctx (tCtxLambda_l _ tCtxHole _)).
+  Qed.
+
+  Lemma red_letin_alt Γ na d0 d1 t0 t1 b0 b1 :
+    red Σ Γ d0 d1 -> red Σ Γ t0 t1 -> red Σ (Γ ,, vdef na d0 t0) b0 b1 ->
+    red Σ Γ (tLetIn na d0 t0 b0) (tLetIn na d1 t1 b1).
+  Proof.
+    intros; eapply (transitivity (y := tLetIn na d0 t0 b1)).
+    now eapply (red_ctx (tCtxLetIn_r _ _ _ tCtxHole)).
+    eapply (transitivity (y := tLetIn na d0 t1 b1)).
+    now eapply (red_ctx (tCtxLetIn_b _ _ tCtxHole _)).
+    now apply (red_ctx (tCtxLetIn_l _ tCtxHole _ _)).
+  Qed.
+
+  (** Parallel reduction is included in the reflexive transitive closure of 1-step reduction *)
+  Lemma pred1_red Γ Γ' : forall M N, pred1 Σ Γ Γ' M N -> red Σ Γ M N.
+  Proof.
+    revert Γ Γ'. eapply (@pred1_ind_all_ctx Σ _
+                                            (fun Γ Γ' =>
+       All2_local_env (on_decl (fun Γ Γ' M N => pred1 Σ Γ Γ' M N -> red Σ Γ M N)) Γ Γ')%type);
+                   intros; try constructor; pcuic.
+    eapply All2_local_env_impl; eauto.
+    - (* Contexts *)
+      unfold on_decl => Δ Δ' t T U Hlen.
+      destruct t; auto.
+      destruct p; auto. intuition.
+
+    - (* Beta *)
+      apply red_trans with (tApp (tLambda na t0 b1) a0).
+      eapply (@red_app Σ); [apply red_abs|]; auto with pcuic.
+      apply red_trans with (tApp (tLambda na t0 b1) a1).
+      eapply (@red_app Σ); auto with pcuic.
+      apply red1_red. constructor.
+
+    - (* Zeta *)
+      eapply red_trans with (tLetIn na d0 t0 b1).
+      eapply red_letin; eauto with pcuic.
+      eapply red_trans with (tLetIn na d1 t1 b1).
+      eapply red_letin; eauto with pcuic.
+      eapply red1_red; constructor.
+
+    - (* Rel in context *)
+      eapply nth_error_pred1_ctx in X0; eauto.
+      destruct X0 as [body' [Hnth Hpred]].
+      eapply red_trans with (lift0 (S i) body').
+      eapply red1_red; constructor; auto.
+      eapply nth_error_pred1_ctx_all_defs in H; eauto.
+      specialize (Hpred H).
+      rewrite -(firstn_skipn (S i) Γ).
+      eapply weakening_red_0 => //.
+      rewrite firstn_length_le //.
+      destruct nth_error eqn:Heq.
+      eapply nth_error_Some_length in Heq. lia. noconf Hnth.
+
+    - (* Iota *)
+      transitivity (tCase (ind, pars) p (mkApps (tConstruct ind c u) args1) brs1).
+      eapply red_case; auto.
+      eapply red_mkApps. auto. solve_all. red in X2; solve_all.
+      eapply red1_red. constructor.
+
+    - move: H H0.
+      move => unf isc.
+      transitivity (mkApps (tFix mfix1 idx) args1).
+      eapply red_mkApps. eapply red_fix_congr. red in X3. solve_all. eapply a.
+      solve_all.
+      eapply red_step. econstructor; eauto. eauto.
+
+    - transitivity (tCase ip p1 (mkApps (tCoFix mfix1 idx) args1) brs1).
+      eapply red_case; eauto.
+      eapply red_mkApps; [|solve_all].
+      eapply red_cofix_congr. red in X3; solve_all. eapply a0.
+      red in X7; solve_all.
+      eapply red_step. econstructor; eauto. eauto.
+
+    - transitivity (tProj p (mkApps (tCoFix mfix1 idx) args1)).
+      eapply red_proj_congr; eauto.
+      eapply red_mkApps; [|solve_all].
+      eapply red_cofix_congr. red in X3; solve_all. eapply a.
+      eapply red_step. econstructor; eauto. eauto.
+
+    - eapply red1_red. econstructor; eauto.
+
+    - transitivity (tProj (i, pars, narg) (mkApps (tConstruct i k u) args1)).
+      eapply red_proj_congr; eauto.
+      eapply red_mkApps; [|solve_all]. auto.
+      eapply red1_red. econstructor; eauto.
+
+    - now eapply red_abs_alt.
+    - now eapply red_app.
+    - now eapply red_letin_alt => //.
+    - eapply red_case => //. red in X3; solve_all.
+    - now eapply red_proj_congr.
+    - eapply red_fix_congr. red in X3; solve_all. eapply a.
+    - eapply red_cofix_congr. red in X3; solve_all. eapply a.
+    - eapply red_prod; auto.
+    - eapply red_evar; auto. solve_all.
+  Qed.
+
+End PredRed.
+
+Lemma clos_t_rt {A} {R : A -> A -> Type} x y : trans_clos R x y -> clos_refl_trans R x y.
+Proof.
+  induction 1; try solve [econstructor; eauto].
+Qed.
+
+Require Import CMorphisms.
+
+Section AbstractConfluence.
+  Section Diamond.
+    Context {A : Type} (R : A -> A -> Type).
+    Definition joinable (x y : A) := ∑ z, R x z * R y z.
+    Definition diamond := forall x y z, R x y -> R x z -> joinable y z.
+  End Diamond.
+
+  Definition confluent {A} (R : relation A) := diamond (clos_refl_trans R).
+
+  Instance joinable_proper A : CMorphisms.Proper (relation_equivalence ==> relation_equivalence)%signature (@joinable A).
+  Proof.
+    reduce_goal. split; unfold joinable; intros.
+    destruct X0. exists x1. intuition eauto. setoid_rewrite (X x0 x1) in a. auto.
+    specialize (X y0 x1). now apply X in b.
+    red in X.
+    destruct X0 as [z [rl rr]].
+    apply X in rl. apply X in rr.
+    exists z; split; auto.
+  Qed.
+
+  Instance diamond_proper A : CMorphisms.Proper (relation_equivalence ==> iffT)%signature (@diamond A).
+  Proof.
+    reduce_goal.
+    rewrite /diamond.
+    split; intros.
+    setoid_rewrite <- (X x0 y0) in X1.
+    setoid_rewrite <- (X x0 z) in X2.
+    specialize (X0 _ _ _ X1 X2).
+    pose (joinable_proper _ _ _ X).
+    now apply r in X0.
+    setoid_rewrite (X x0 y0) in X1.
+    setoid_rewrite (X x0 z) in X2.
+    specialize (X0 _ _ _ X1 X2).
+    pose (joinable_proper _ _ _ X).
+    now apply r in X0.
+  Qed.
+
+  Lemma clos_rt_proper A : CMorphisms.Proper (relation_equivalence ==> relation_equivalence) (@clos_refl_trans A).
+  Proof.
+    reduce_goal. split; intros.
+    induction X0; try apply X in r; try solve [econstructor; eauto].
+    induction X0; try apply X in r; try solve [econstructor; eauto].
+  Qed.
+
+  Instance confluent_proper A : CMorphisms.Proper (relation_equivalence ==> iffT)%signature (@confluent A).
+  Proof.
+    reduce_goal.
+    split; rewrite /confluent; auto.
+    pose proof (diamond_proper A). apply X0. apply clos_rt_proper.
+    now symmetry.
+    pose proof (diamond_proper A). apply X0. apply clos_rt_proper.
+    now symmetry.
+  Qed.
+
+  Definition clos_rt_monotone {A} (R S : relation A) :
+    inclusion R S -> inclusion (clos_refl_trans R) (clos_refl_trans S).
+  Proof.
+    move => incls x y.
+    induction 1; solve [econstructor; eauto].
+  Qed.
+
+  Lemma relation_equivalence_inclusion {A} (R S : relation A) :
+    inclusion R S -> inclusion S R -> relation_equivalence R S.
+  Proof. firstorder. Qed.
+
+  Lemma sandwich {A} (R S : A -> A -> Type) :
+    inclusion R S -> inclusion S (clos_refl_trans R) ->
+    (iffT (confluent S) (confluent R)).
+  Proof.
+    intros inclR inclS.
+    apply clos_rt_monotone in inclR.
+    apply clos_rt_monotone in inclS.
+    assert (inclusion (clos_refl_trans S) (clos_refl_trans R)).
+    etransitivity; eauto.
+    apply clos_rt_idempotent.
+    rewrite /confluent.
+    apply diamond_proper.
+    now apply relation_equivalence_inclusion.
+  Qed.
+
+  Lemma clos_rt_t_incl {A} {R : relation A} `{Reflexive A R} :
+    inclusion (clos_refl_trans R) (trans_clos R).
+  Proof.
+    intros x y. induction 1; try solve [econstructor; eauto].
+  Qed.
+
+  Lemma clos_t_rt_incl {A} {R : relation A} `{Reflexive A R} :
+    inclusion (trans_clos R) (clos_refl_trans R).
+  Proof.
+    intros x y. induction 1; try solve [econstructor; eauto].
+  Qed.
+
+  Lemma clos_t_rt_equiv {A} {R} `{Reflexive A R} :
+    relation_equivalence (trans_clos R) (clos_refl_trans R).
+  Proof.
+    apply relation_equivalence_inclusion.
+    apply clos_t_rt_incl.
+    apply clos_rt_t_incl.
+  Qed.
+
+End AbstractConfluence.
+
+Unset Universe Minimization ToSet.
+
+Section RedConfluence.
+  Context {Σ} (wfΣ : wf Σ).
+
+  Instance pred1_refl Γ : Reflexive (pred1 Σ Γ Γ).
+  Proof. red; apply pred1_refl. Qed.
+
+  Definition pred1_rel : (context * term) -> (context * term) -> Type :=
+    fun t u => pred1 Σ (fst t) (fst u) (snd t) (snd u).
+
+  Instance pred1_rel_refl : Reflexive pred1_rel.
+  Proof. red. intros [ctx x]. red. simpl. apply pred1_refl. Qed.
+
+  Lemma red1_weak_confluence Γ t u v :
+    red1 Σ Γ t u -> red1 Σ Γ t v ->
+    ∑ t', red Σ Γ u t' * red Σ Γ v t'.
+  Proof.
+    move/(red1_pred1 wfΣ) => tu.
+    move/(red1_pred1 wfΣ) => tv.
+    eapply confluence in tu; eauto.
+    destruct tu as [redl redr].
+    eapply pred1_red in redl; auto.
+    eapply pred1_red in redr; auto.
+    eexists _; split; eauto.
+  Qed.
+
+  Lemma sc_pred1_rel t u v :
+    pred1_rel t u -> pred1_rel t v ->
+    ∑ t', pred1_rel u t' * pred1_rel v t'.
+  Proof.
+    move=> tu tv.
+    destruct (confluence _ _ _ _ _ _ _ wfΣ tu tv).
+    eexists (rho_ctx Σ (fst t), rho Σ (rho_ctx Σ (fst t)) (snd t)).
+    split; auto.
+  Qed.
+
+  Lemma pred1_rel_trans_pred1_confluent t u v :
+    trans_clos_1n pred1_rel t u ->
+    pred1_rel t v ->
+    ∑ t', trans_clos_1n pred1_rel u t' * trans_clos_1n pred1_rel v t'.
+  Proof.
+    move => tu.
+    revert v.
+    induction tu.
+    intros.
+    - destruct (sc_pred1_rel _ _ _ r X); auto.
+      eexists; split; constructor; intuition eauto.
+    - move => v xv.
+      destruct (sc_pred1_rel _ _ _ r xv); auto.
+      destruct p. specialize (IHtu _ p).
+      destruct IHtu as [nf [redl redr]].
+      exists nf. split; auto.
+      econstructor 2; eauto.
+  Qed.
+
+  Lemma pred1_rel_t1n_confluent {t u v} :
+    trans_clos_1n pred1_rel t u ->
+    trans_clos_1n pred1_rel t v ->
+    ∑ t', trans_clos_1n pred1_rel u t' * trans_clos_1n pred1_rel v t'.
+  Proof.
+    move => tu tv.
+    induction tv in u, tu |- *.
+    - eapply pred1_rel_trans_pred1_confluent; eauto.
+    - eapply pred1_rel_trans_pred1_confluent in r; eauto.
+      destruct r as [nf [redl redr]].
+      specialize (IHtv _ redr) as [nf' [redl' redr']].
+      exists nf'; intuition auto.
+      apply trans_clos_t1n_iff.
+      econstructor 2; eapply trans_clos_t1n_iff; eauto.
+  Qed.
+
+  Lemma pred1_rel_tclos_confluent {t u v} :
+    trans_clos pred1_rel t u ->
+    trans_clos pred1_rel t v ->
+    ∑ t', trans_clos pred1_rel u t' * trans_clos pred1_rel v t'.
+  Proof.
+    move => tu tv.
+    apply trans_clos_t1n_iff in tu;
+      apply trans_clos_t1n_iff in tv.
+    destruct (pred1_rel_t1n_confluent tu tv).
+    exists x. split; apply trans_clos_t1n_iff; intuition auto.
+  Qed.
+
+  Lemma pred1_rel_confluent : confluent pred1_rel.
+  Proof.
+    move=> x y z H H'.
+    pose proof (pred1_rel_refl).
+    apply (clos_rt_t_incl (H:=X)) in H.
+    apply (clos_rt_t_incl (H:=X)) in H'.
+    pose proof (clos_t_rt_equiv (R:=pred1_rel)).
+    apply (joinable_proper _ _ _ X0).
+    apply (pred1_rel_tclos_confluent H H').
+  Qed.
+
+  Lemma red_trans_clos_pred1 Γ t u :
+    red Σ Γ t u ->
+    trans_clos pred1_rel (Γ, t) (Γ, u).
+  Proof.
+    move/(equiv _ _ (red_alt _ _ _ _)) => tu.
+    induction tu.
+    constructor. now eapply red1_pred1 in r.
+    constructor. pcuic.
+    econstructor 2; eauto.
+  Qed.
+
+  Lemma trans_clos_pred1_red Γ Δ t u :
+    trans_clos (pred1 Σ Γ Δ) t u ->
+    red Σ Γ t u.
+  Proof.
+    move=> H.
+    apply trans_clos_t1n_iff in H.
+    depind H.
+    - eapply pred1_red; eauto.
+    - eapply red_trans with y; auto.
+      eapply pred1_red in r; eauto.
+  Qed.
+
+  Definition on_one_decl (P : context → term → term → Type) (Γ : context) (b : option (term × term)) (t t' : term) :=
+    match b with
+    | Some (b0, b') => ((P Γ b0 b' * (t = t')) + (P Γ t t' * (b0 = b')))%type
+    | None => P Γ t t'
+    end.
+
+  Section OnOne_local_2.
+    Context (P : forall (Γ : context), option (term * term) -> term -> term -> Type).
+
+    Inductive OnOne2_local_env : context -> context -> Type :=
+    | localenv2_cons_abs Γ na t t' :
+        P Γ None t t' ->
+        OnOne2_local_env (Γ ,, vass na t) (Γ ,, vass na t')
+    | localenv2_cons_def Γ na b b' t t' :
+        P Γ (Some (b, b')) t t' ->
+        OnOne2_local_env (Γ ,, vdef na b t) (Γ ,, vdef na b' t')
+    | localenv2_cons_tl Γ Γ' d :
+        OnOne2_local_env Γ Γ' ->
+        OnOne2_local_env (Γ ,, d) (Γ' ,, d).
+  End OnOne_local_2.
+
+  Definition red1_ctx := (OnOne2_local_env (on_one_decl (fun Δ t t' => red1 Σ Δ t t'))).
+
+  Definition red1_rel : relation (context * term) :=
+    relation_disjunction (fun '(Γ, t) '(Δ, u) => (red1 Σ Γ t u * (Γ = Δ)))%type
+                         (fun '(Γ, t) '(Δ, u) => (red1_ctx Γ Δ * (t = u)))%type.
+
+  Definition red_ctx : relation context :=
+    All2_local_env (on_decl (fun Γ Δ t u => red Σ Γ t u)).
+
+
+  Lemma red1_ctx_pred1_ctx Γ Γ' : red1_ctx Γ Γ' -> pred1_ctx Σ Γ Γ'.
+  Proof.
+    intros. induction X; try constructor. pcuic. red. pcuic.
+    now eapply red1_pred1. pcuic.
+    destruct p as [[redb ->]|[redt ->]].
+    - split; pcuic. now eapply red1_pred1.
+    - split; pcuic. now eapply red1_pred1.
+    - destruct d as [na [b|] ty].
+      * constructor; intuition auto. red.
+        split; now eapply pred1_refl_gen.
+      * constructor; intuition auto. red.
+        now eapply pred1_refl_gen.
+  Qed.
+
+  Lemma pred1_ctx_red_ctx Γ Γ' : pred1_ctx Σ Γ Γ' -> red_ctx Γ Γ'.
+  Proof.
+    intros. induction X; try constructor; pcuic.
+    now eapply pred1_red in p.
+    destruct p as [redb redt].
+    split. now apply pred1_red in redb.
+    now apply pred1_red in redt.
+  Qed.
+
+  Definition red_rel' :=
+    fun '(Γ, t) '(Δ, u) =>
+      (red Σ Γ t u * red_ctx Γ Δ)%type.
+
+  Lemma pred1_red' Γ Γ' : forall M N, pred1 Σ Γ Γ' M N -> red_rel' (Γ, M) (Γ', N).
+  Proof.
+    intros * Hred.
+    split. apply (pred1_red wfΣ _ _ _ _ Hred).
+    eapply pred1_pred1_ctx in Hred.
+    now eapply pred1_ctx_red_ctx.
+  Qed.
+
+  Lemma clos_rt_disjunction_left {A} (R S : relation A) :
+    inclusion (clos_refl_trans R)
+              (clos_refl_trans (relation_disjunction R S)).
+  Proof.
+    apply clos_rt_monotone.
+    intros x y H; left; exact H.
+  Qed.
+
+  Lemma clos_rt_disjunction_right {A} (R S : relation A) :
+    inclusion (clos_refl_trans S)
+              (clos_refl_trans (relation_disjunction R S)).
+  Proof.
+    apply clos_rt_monotone.
+    intros x y H; right; exact H.
+  Qed.
+
+  Instance clos_rt_trans A R : Transitive (@clos_refl_trans A R).
+  Proof.
+    intros x y z H H'. now econstructor 3.
+  Qed.
+
+  Instance clos_rt_refl A R : Reflexive (@clos_refl_trans A R).
+  Proof. intros x. constructor 2. Qed.
+
+  Lemma clos_refl_trans_prod_l {A B} (R : relation A) (S : relation (A * B)) :
+    (forall x y b, R x y -> S (x, b) (y, b)) ->
+    forall (x y : A) b,
+      clos_refl_trans R x y ->
+      clos_refl_trans S (x, b) (y, b).
+  Proof.
+    intros. induction X0; try solve [econstructor; eauto].
+  Qed.
+
+  Lemma clos_refl_trans_prod_r {A B} (R : relation B) (S : relation (A * B)) a :
+    (forall x y, R x y -> S (a, x) (a, y)) ->
+    forall (x y : B),
+      clos_refl_trans R x y ->
+      clos_refl_trans S (a, x) (a, y).
+  Proof.
+    intros. induction X0; try solve [econstructor; eauto].
+  Qed.
+
+  Lemma clos_rt_OnOne2_local_env_incl R :
+    inclusion (OnOne2_local_env (on_one_decl (fun Δ => clos_refl_trans (R Δ))))
+              (clos_refl_trans (OnOne2_local_env (on_one_decl R))).
+  Proof.
+    intros x y H.
+    induction H; firstorder.
+    - red in p.
+      induction p. repeat constructor. firstorder.
+      constructor 2.
+      etransitivity; eauto.
+    - subst.
+      induction a. repeat constructor. firstorder.
+      constructor 2.
+      etransitivity; eauto.
+    - subst.
+      induction a. constructor. constructor. red. right. firstorder.
+      constructor 2.
+      etransitivity; eauto.
+    - clear H. induction IHOnOne2_local_env. constructor. now constructor 3.
+      constructor 2.
+      etransitivity; eauto.
+  Qed.
+
+  Lemma OnOne2_local_env_impl R S :
+    (forall Δ, inclusion (R Δ) (S Δ)) ->
+    inclusion (OnOne2_local_env (on_one_decl R))
+              (OnOne2_local_env (on_one_decl S)).
+  Proof.
+    intros H x y H'.
+    induction H'; try solve [econstructor; firstorder].
+  Qed.
+
+  Lemma red_ctx_clos_rt_red1_ctx : inclusion red_ctx (clos_refl_trans red1_ctx).
+  Proof.
+    intros x y H.
+    induction H; try firstorder.
+    red in p.
+    transitivity (Γ ,, vass na t').
+    eapply clos_rt_OnOne2_local_env_incl. constructor. red.
+    eapply red_alt in p; eauto.
+    clear p H.
+    induction IHAll2_local_env. constructor. constructor 3. apply r.
+    constructor 2.
+    etransitivity; eauto.
+
+    apply red_alt in a. apply red_alt in b0.
+    transitivity (Γ ,, vdef na b t').
+    - eapply clos_rt_OnOne2_local_env_incl. constructor 2. red.
+      right. split; auto.
+    - transitivity (Γ ,, vdef na b' t').
+      eapply clos_rt_OnOne2_local_env_incl.
+      constructor 2. red. left; split; auto.
+      clear -IHAll2_local_env.
+      induction IHAll2_local_env.
+      * constructor. now constructor.
+      * constructor 2.
+      * etransitivity; eauto.
+  Qed.
+
+  Lemma clos_rt_red1_rel_red_rel : inclusion red_rel' (clos_refl_trans red1_rel).
+  Proof.
+    move=> [Γ t] [Δ u] [redt redctx].
+    eapply red_alt in redt.
+    eapply clos_rt_rt1n_iff in redt.
+    induction redt.
+    induction redctx; try solve [constructor; eauto].
+    - red in p.
+      etransitivity.
+      * eapply clos_rt_disjunction_right.
+        eapply red_alt in p. instantiate (1:= (Γ',, vass na t', x)).
+        eapply clos_refl_trans_prod_l. intros. split; eauto.
+        apply red_ctx_clos_rt_red1_ctx. constructor; auto.
+        red. apply red_alt; auto.
+      * clear p. eapply clos_rt_disjunction_right.
+        eapply clos_refl_trans_prod_l. intros. split; eauto.
+        constructor 2.
+    - red in p.
+      destruct p.
+      eapply red_alt in r. eapply red_alt in r0.
+      etransitivity.
+      * eapply clos_rt_disjunction_right.
+        instantiate (1:= (Γ',, vdef na b' t', x)).
+        eapply clos_refl_trans_prod_l. intros. split; eauto.
+        apply red_ctx_clos_rt_red1_ctx. constructor; auto.
+        red. split; apply red_alt; auto.
+      * clear r r0.
+        eapply clos_rt_disjunction_right.
+        eapply clos_refl_trans_prod_l. intros. split; eauto.
+        constructor 2.
+    - transitivity (Γ, y).
+      * eapply clos_rt_disjunction_left.
+        eapply clos_refl_trans_prod_r. intros. split; eauto.
+        constructor. apply r.
+      * assumption.
+  Qed.
+
+  Lemma pred_rel_confluent : confluent red1_rel.
+  Proof.
+    notypeclasses refine (fst (sandwich _ _ _ _) _).
+    3:eapply pred1_rel_confluent; eauto.
+    intros [ctx t] [ctx' t'].
+    rewrite /red1_rel /pred1_rel /=.
+    intros [[l <-]|[r <-]].
+    - now eapply red1_pred1.
+    - eapply pred1_refl_gen. now apply red1_ctx_pred1_ctx.
+    - intros x y pred. red in pred.
+      eapply pred1_red' in pred; auto.
+      destruct pred.
+      destruct x, y. simpl in *.
+      transitivity (c, t0).
+      eapply clos_rt_disjunction_left.
+      eapply clos_refl_trans_prod_r. intros. split; eauto.
+      now eapply red_alt in r.
+      eapply clos_rt_disjunction_right.
+      eapply clos_refl_trans_prod_l. intros. split; eauto.
+      now eapply red_ctx_clos_rt_red1_ctx.
+  Qed.
+
+  Lemma clos_refl_trans_out Γ x y :
+    clos_refl_trans (red1 Σ Γ) x y -> clos_refl_trans red1_rel (Γ, x) (Γ, y).
+  Proof.
+    induction 1. constructor. red. left. firstorder.
+    constructor 2.
+    econstructor 3; eauto.
+  Qed.
+
+  Lemma clos_red_rel_out x y :
+    clos_refl_trans red1_rel x y ->
+    clos_refl_trans pred1_rel x y.
+  Proof.
+    eapply clos_rt_monotone. clear x y.
+    intros [Γ t] [Δ u] hred.
+    destruct hred as [[ht eq]|[hctx eq]]. subst.
+    red. simpl. now eapply red1_pred1.
+    subst. red.
+    simpl.
+    eapply pred1_refl_gen. now eapply red1_ctx_pred1_ctx.
+  Qed.
+
+  (* Lemma clos_red_rel_out' x y : *)
+  (*   clos_refl_trans red1_rel x y -> *)
+  (*   clos_refl_trans (red1 Σ (fst y)) (snd x) (snd y). *)
+  (* Proof. *)
+  (*   intros H. eapply clos_red_rel_out in H. *)
+  (*   destruct x, y. simpl in *. *)
+  (*   induction H. red in r. *)
+
+
+  (*   eapply clos_rt_red1_rel_red_rel. *)
+
+  (*   eapply clos_rt_rt1n in H. *)
+  (*   induction H; try destruct x as [Γ t]; try destruct y as [Δ u]; simpl in *. *)
+  (*   - constructor 2. *)
+  (*   - destruct z as [? ?]. *)
+  (*     simpl in *. intros <-. *)
+  (*     red in r. *)
+  (*     destruct r. *)
+  (*     * destruct p. subst. *)
+  (*       eapply clos_rt1n_rt. econstructor; eauto. *)
+  (*       eapply clos_rt_rt1n. *)
+  (*       now eapply IHclos_refl_trans_1n. *)
+  (*     * destruct p. *)
+  (*       subst. *)
+  (* Qed. *)
+
+  Lemma red1_confluent Γ : confluent (red1 Σ Γ).
+  Proof.
+    intros x y z.
+    intros.
+    pose proof (pred_rel_confluent (Γ, x) (Γ, y) (Γ, z)).
+    forward X1 by now eapply clos_refl_trans_out.
+    forward X1 by now eapply clos_refl_trans_out.
+    destruct X1 as [[Δ nf] [redl redr]].
+    exists nf. split.
+    eapply clos_red_rel_out in redl.
+    eapply clos_red_rel_out in redr.
+  Abort.
+
+End RedConfluence.
