pcuic/theories/TemplateToPCUICCorrectness.v
@@ -709,7 +709,8 @@ Proof.
 
   - constructor. solve_all. solve_all.
     apply OnOne2_map. apply (OnOne2_All_mix_left H1) in X. clear H1.
-    solve_all. red. simpl. apply b1. solve_all. simpl. auto.
+    solve_all. red. simpl. simpl in *. split; auto. apply b1. solve_all. simpl. auto.
+    admit. (* Need to update template-coq's red1 with annotation preservation *)
 
   - rewrite !trans_mkApps; auto with wf. eapply wf_red1 in X; auto.
     apply PCUICSubstitution.red1_mkApps_l. auto.
@@ -732,7 +733,8 @@ Proof.
     apply (OnOne2_All_mix_left Hwf) in X. clear Hwf.
     solve_all.
     red. rewrite <- !map_dtype. rewrite <- !map_dbody. intuition eauto.
-    eapply b0; solve_all; eauto. rewrite b. auto.
+    eapply b0; solve_all; eauto. rewrite b. auto. simpl.
+    admit. (* Annotation preservation *)
 
   - apply fix_red_body. apply OnOne2_map. repeat toAll.
     apply (OnOne2_All_mix_left Hwf) in X. clear Hwf.
@@ -750,14 +752,14 @@ Proof.
     eapply (refine_red1_Γ); [|apply b0].
     f_equal. f_equal. apply mapi_ext; intros [] [].
     rewrite lift0_p. simpl. rewrite LiftSubst.lift0_p. reflexivity.
-    rewrite trans_lift. simpl. reflexivity.
-    now rewrite b.
+    rewrite trans_lift. simpl. reflexivity. simpl.
+    rewrite b. admit.
 
   - constructor. solve_all. apply OnOne2_map. repeat toAll.
     apply (OnOne2_All_mix_left Hwf) in X. clear Hwf.
     solve_all.
     red. rewrite <- !map_dtype. rewrite <- !map_dbody. intuition eauto.
-    apply b0. toAll. auto. auto. rewrite b. auto.
+    apply b0. toAll. auto. auto. rewrite b. auto. simpl. admit.
 
   - apply cofix_red_body. apply OnOne2_map. repeat toAll.
     apply (OnOne2_All_mix_left Hwf) in X. clear Hwf.
@@ -775,9 +777,9 @@ Proof.
     eapply (refine_red1_Γ); [|apply b0].
     f_equal. f_equal. apply mapi_ext; intros [] [].
     rewrite lift0_p. simpl. rewrite LiftSubst.lift0_p. reflexivity.
-    rewrite trans_lift. simpl. reflexivity.
-    now rewrite b.
-Qed.
+    rewrite trans_lift. simpl. reflexivity. simpl.
+    rewrite b. admit.
+Admitted.
 
 Lemma trans_cumul Σ Γ T U :
   TTy.on_global_env (fun Σ Γ t T => match t with Some b => Ast.wf b /\ Ast.wf T | None => Ast.wf T end) Σ ->
